general code refactoring and lambda specialization

Tests/Basic.lean
@@ -210,6 +210,438 @@ fun {α} [SlowEnum α] f => List.foldl (fun acc x => acc + f x) 0 univSlow -/
 #guard_msgs in
 #print genericSum._spec
 
+/-! More involved regression tests for traversal and proof construction. -/
+
+def nestedLetDeep (x : Nat) :=
+  let a := 0 + x
+  let b := 0 + a + 1
+  let c := b + (0 + a)
+  c + (0 + b)
+
+#sas (config := { zeta := false }) nestedLetDeep
+/--
+info: def LeanSASTests.nestedLetDeep._spec : Nat → Nat :=
+fun x =>
+  let a := x;
+  let b := a + 1;
+  let c := b + a;
+  c + b
+-/
+#guard_msgs in
+#print nestedLetDeep._spec
+/-- info: LeanSASTests.nestedLetDeep._spec.eq_thm (x : Nat) : nestedLetDeep._spec x = nestedLetDeep x -/
+#guard_msgs in
+#check nestedLetDeep._spec.eq_thm
+
+example (x : Nat) : nestedLetDeep._spec x = nestedLetDeep x :=
+  nestedLetDeep._spec.eq_thm x
+
+def lambdaCallee (k x : Nat) := k + x
+
+def lambdaTransform (k : Nat) : Nat → Nat :=
+  fun x => lambdaCallee (0 + k) (0 + x)
+
+#sas lambdaTransform
+/-- info: def LeanSASTests.lambdaTransform._spec : Nat → Nat → Nat :=
+fun k a => lambdaCallee._spec k a -/
+#guard_msgs in
+#print lambdaTransform._spec
+/-- info: def LeanSASTests.lambdaCallee._spec : Nat → Nat → Nat :=
+fun x x_1 => x + x_1 -/
+#guard_msgs in
+#print lambdaCallee._spec
+/-- info: LeanSASTests.lambdaTransform._spec.eq_thm (k a✝ : Nat) : lambdaTransform._spec k a✝ = lambdaTransform k a✝ -/
+#guard_msgs in
+#check lambdaTransform._spec.eq_thm
+
+example (k x : Nat) : lambdaTransform._spec k x = lambdaTransform k x :=
+  lambdaTransform._spec.eq_thm k x
+
+def appArgCallee (n : Nat) (b : Bool) :=
+  if b then n + 1 else n
+
+def appArgTransform (x : Nat) (b : Bool) :=
+  appArgCallee (0 + x) (!(!b))
+
+#sas appArgTransform
+/-- info: def LeanSASTests.appArgTransform._spec : Nat → Bool → Nat :=
+fun x b => appArgCallee._spec x b -/
+#guard_msgs in
+#print appArgTransform._spec
+/-- info: def LeanSASTests.appArgCallee._spec : Nat → Bool → Nat :=
+fun x x_1 => if x_1 = true then x + 1 else x -/
+#guard_msgs in
+#print appArgCallee._spec
+/-- info: LeanSASTests.appArgTransform._spec.eq_thm (x : Nat) (b : Bool) : appArgTransform._spec x b = appArgTransform x b -/
+#guard_msgs in
+#check appArgTransform._spec.eq_thm
+
+example (x : Nat) (b : Bool) : appArgTransform._spec x b = appArgTransform x b :=
+  appArgTransform._spec.eq_thm x b
+
+def functionArgCallee (f : Nat → Nat) (x : Nat) :=
+  f x
+
+def functionArgTransform (x z : Nat) :=
+  functionArgCallee (fun y => 0 + y*z + x) x
+
+#sas functionArgTransform
+/-- info: def LeanSASTests.functionArgTransform._spec : Nat → Nat → Nat :=
+fun x z => functionArgCallee_sas_1 x z -/
+#guard_msgs in
+#print functionArgTransform._spec
+/-- info: def LeanSASTests.functionArgCallee_sas_1 : Nat → Nat → Nat :=
+fun x x_1 => x * x_1 + x -/
+#guard_msgs in
+#print functionArgCallee_sas_1
+/-- info: LeanSASTests.functionArgTransform._spec.eq_thm (x z : Nat) : functionArgTransform._spec x z = functionArgTransform x z -/
+#guard_msgs in
+#check functionArgTransform._spec.eq_thm
+
+example (x z : Nat) : functionArgTransform._spec x z = functionArgTransform x z :=
+  functionArgTransform._spec.eq_thm x z
+
+
+def functionArg2Callee (f : Nat → Nat → Nat) (x y : Nat) :=
+  f (x+y) (x*y)
+
+def functionArg2Transform (x z : Nat) :=
+  functionArg2Callee (fun y => Nat.add (0 + y*z + x)) x
+
+#sas functionArg2Transform
+/--
+info: def LeanSASTests.functionArg2Transform._spec : Nat → Nat → Nat → Nat :=
+fun x z y => functionArg2Callee_sas_1 x z y
+-/
+#guard_msgs in
+#print functionArg2Transform._spec
+
+/--
+info: def LeanSASTests.functionArg2Callee_sas_1 : Nat → Nat → Nat → Nat :=
+fun x x_1 x_2 => (x + x_2) * x_1 + x + x * x_2
+-/
+#guard_msgs in
+#print functionArg2Callee_sas_1
+
+def expensiveInput (x : Nat) :=
+  x + 1
+
+def nonlinearFunctionArgCallee (f : Nat → Nat) (x : Nat) :=
+  f (expensiveInput x)
+
+def nonlinearFunctionArgTransform (a b x : Nat) :=
+  nonlinearFunctionArgCallee (fun y => a * y + b * y) x
+
+#sas (config := { zeta := false }) nonlinearFunctionArgTransform
+/--
+info: def LeanSASTests.nonlinearFunctionArgTransform._spec : Nat → Nat → Nat → Nat :=
+fun a b x => nonlinearFunctionArgCallee_sas_1 a b x
+-/
+#guard_msgs in
+#print nonlinearFunctionArgTransform._spec
+/--
+info: def LeanSASTests.nonlinearFunctionArgCallee_sas_1 : Nat → Nat → Nat → Nat :=
+fun x x_1 x_2 =>
+  let y := expensiveInput._spec x_2;
+  x * y + x_1 * y
+-/
+#guard_msgs in
+#print nonlinearFunctionArgCallee_sas_1
+/--
+info: LeanSASTests.nonlinearFunctionArgTransform._spec.eq_thm (a b x : Nat) :
+  nonlinearFunctionArgTransform._spec a b x = nonlinearFunctionArgTransform a b x
+-/
+#guard_msgs in
+#check nonlinearFunctionArgTransform._spec.eq_thm
+
+example (a b x : Nat) :
+    nonlinearFunctionArgTransform._spec a b x = nonlinearFunctionArgTransform a b x :=
+  nonlinearFunctionArgTransform._spec.eq_thm a b x
+
+def captureOrderCallee (n : Nat) (f : Nat → Nat) (m : Nat) :=
+  f n + m
+
+def captureOrderTransform (x y z : Nat) :=
+  captureOrderCallee z (fun w => x + w + y) x
+
+#sas captureOrderTransform
+/-- info: def LeanSASTests.captureOrderTransform._spec : Nat → Nat → Nat → Nat :=
+fun x y z => captureOrderCallee_sas_1 z x y -/
+#guard_msgs in
+#print captureOrderTransform._spec
+/-- info: def LeanSASTests.captureOrderCallee_sas_1 : Nat → Nat → Nat → Nat :=
+fun x x_1 x_2 => x_1 + x + x_2 + x_1 -/
+#guard_msgs in
+#print captureOrderCallee_sas_1
+/--
+info: LeanSASTests.captureOrderTransform._spec.eq_thm (x y z : Nat) :
+  captureOrderTransform._spec x y z = captureOrderTransform x y z
+-/
+#guard_msgs in
+#check captureOrderTransform._spec.eq_thm
+
+example (x y z : Nat) : captureOrderTransform._spec x y z = captureOrderTransform x y z :=
+  captureOrderTransform._spec.eq_thm x y z
+
+def repeatedCaptureCallee (f : Nat → Nat) (x : Nat) :=
+  f x
+
+def repeatedCaptureTransform (a x : Nat) :=
+  repeatedCaptureCallee (fun y => a + y + a) x
+
+#sas repeatedCaptureTransform
+/-- info: def LeanSASTests.repeatedCaptureTransform._spec : Nat → Nat → Nat :=
+fun a x => repeatedCaptureCallee_sas_1 a x -/
+#guard_msgs in
+#print repeatedCaptureTransform._spec
+/-- info: def LeanSASTests.repeatedCaptureCallee_sas_1 : Nat → Nat → Nat :=
+fun x x_1 => x + x_1 + x -/
+#guard_msgs in
+#print repeatedCaptureCallee_sas_1
+/--
+info: LeanSASTests.repeatedCaptureTransform._spec.eq_thm (a x : Nat) :
+  repeatedCaptureTransform._spec a x = repeatedCaptureTransform a x
+-/
+#guard_msgs in
+#check repeatedCaptureTransform._spec.eq_thm
+
+example (a x : Nat) : repeatedCaptureTransform._spec a x = repeatedCaptureTransform a x :=
+  repeatedCaptureTransform._spec.eq_thm a x
+
+def cheapBetaCallee (f : Nat → Nat) (x : Nat) :=
+  f x
+
+def cheapBetaTransform (a x : Nat) :=
+  cheapBetaCallee (fun y => y + y + a) x
+
+#sas (config := { zeta := false }) cheapBetaTransform
+/-- info: def LeanSASTests.cheapBetaTransform._spec : Nat → Nat → Nat :=
+fun a x => cheapBetaCallee_sas_1 a x -/
+#guard_msgs in
+#print cheapBetaTransform._spec
+/-- info: def LeanSASTests.cheapBetaCallee_sas_1 : Nat → Nat → Nat :=
+fun x x_1 => x_1 + x_1 + x -/
+#guard_msgs in
+#print cheapBetaCallee_sas_1
+/-- info: LeanSASTests.cheapBetaTransform._spec.eq_thm (a x : Nat) : cheapBetaTransform._spec a x = cheapBetaTransform a x -/
+#guard_msgs in
+#check cheapBetaTransform._spec.eq_thm
+
+example (a x : Nat) : cheapBetaTransform._spec a x = cheapBetaTransform a x :=
+  cheapBetaTransform._spec.eq_thm a x
+
+def todoArgProducer (x : Nat) :=
+  0 + x
+
+def todoArgConsumer (n k : Nat) :=
+  n + k
+
+def todoArgumentSpecialization (x : Nat) :=
+  todoArgConsumer (todoArgProducer x) 5
+
+#sas todoArgumentSpecialization
+/-- info: def LeanSASTests.todoArgumentSpecialization._spec : Nat → Nat :=
+fun x => todoArgConsumer_sas_1 (todoArgProducer._spec x) -/
+#guard_msgs in
+#print todoArgumentSpecialization._spec
+/-- info: def LeanSASTests.todoArgProducer._spec : Nat → Nat :=
+fun x => x -/
+#guard_msgs in
+#print todoArgProducer._spec
+/-- info: def LeanSASTests.todoArgConsumer_sas_1 : Nat → Nat :=
+fun x => x + 5 -/
+#guard_msgs in
+#print todoArgConsumer_sas_1
+/--
+info: LeanSASTests.todoArgumentSpecialization._spec.eq_thm (x : Nat) :
+  todoArgumentSpecialization._spec x = todoArgumentSpecialization x
+-/
+#guard_msgs in
+#check todoArgumentSpecialization._spec.eq_thm
+
+example (x : Nat) : todoArgumentSpecialization._spec x = todoArgumentSpecialization x :=
+  todoArgumentSpecialization._spec.eq_thm x
+
+def affine (a b x : Nat) :=
+  a * x + b
+
+def staticUnderLetLambda (x : Nat) :=
+  let mk := fun y => affine 4 7 (0 + y)
+  let y := 0 + x
+  mk y + mk (0 + y)
+
+#sas (config := { zeta := false }) staticUnderLetLambda
+/--
+info: def LeanSASTests.staticUnderLetLambda._spec : Nat → Nat :=
+fun x =>
+  let mk := fun y => affine_sas_1 y;
+  let y := x;
+  mk y + mk y
+-/
+#guard_msgs in
+#print staticUnderLetLambda._spec
+/-- info: def LeanSASTests.affine_sas_1 : Nat → Nat :=
+fun x => 4 * x + 7 -/
+#guard_msgs in
+#print affine_sas_1
+/-- info: LeanSASTests.staticUnderLetLambda._spec.eq_thm (x : Nat) : staticUnderLetLambda._spec x = staticUnderLetLambda x -/
+#guard_msgs in
+#check staticUnderLetLambda._spec.eq_thm
+
+example (x : Nat) : staticUnderLetLambda._spec x = staticUnderLetLambda x :=
+  staticUnderLetLambda._spec.eq_thm x
+
+structure Pair where
+  left : Nat
+  right : Nat
+
+def pairScore (p : Pair) :=
+  p.left + (0 + p.right)
+
+def projectionTransform (x : Nat) :=
+  let p : Pair := { left := 0 + x, right := x + 1 }
+  pairScore p + (0 + p.left)
+
+#sas (config := { zeta := false }) projectionTransform
+/--
+info: def LeanSASTests.projectionTransform._spec : Nat → Nat :=
+fun x =>
+  let p := { left := x, right := x + 1 };
+  pairScore p + p.left
+-/
+#guard_msgs in
+#print projectionTransform._spec
+/-- info: LeanSASTests.projectionTransform._spec.eq_thm (x : Nat) : projectionTransform._spec x = projectionTransform x -/
+#guard_msgs in
+#check projectionTransform._spec.eq_thm
+
+example (x : Nat) : projectionTransform._spec x = projectionTransform x :=
+  projectionTransform._spec.eq_thm x
+
+def makePairForProjection (x : Nat) : Pair :=
+  { left := 0 + x, right := x + 1 }
+
+def projectionOfTransformedStruct (x : Nat) :=
+  (makePairForProjection x).left
+
+#sas projectionOfTransformedStruct
+/-- info: def LeanSASTests.projectionOfTransformedStruct._spec : Nat → Nat :=
+fun x => (makePairForProjection._spec x).left -/
+#guard_msgs in
+#print projectionOfTransformedStruct._spec
+/-- info: def LeanSASTests.makePairForProjection._spec : Nat → Pair :=
+fun x => { left := x, right := x + 1 } -/
+#guard_msgs in
+#print makePairForProjection._spec
+/--
+info: LeanSASTests.projectionOfTransformedStruct._spec.eq_thm (x : Nat) :
+  projectionOfTransformedStruct._spec x = projectionOfTransformedStruct x
+-/
+#guard_msgs in
+#check projectionOfTransformedStruct._spec.eq_thm
+
+example (x : Nat) :
+    projectionOfTransformedStruct._spec x = projectionOfTransformedStruct x :=
+  projectionOfTransformedStruct._spec.eq_thm x
+
+def genericFoldMap {α : Type} [SlowEnum α] (offset : Nat) (f : α → Nat) : Nat :=
+  ((univSlow (α := α)).map (fun a => 0 + offset + f a)).foldl (fun acc n => acc + n) 0
+
+def smallFoldMap : Nat :=
+  genericFoldMap (α := Small) 5 smallCode
+
+#sas smallFoldMap
+/-- info: def LeanSASTests.smallFoldMap._spec : Nat :=
+genericFoldMap_sas_1 -/
+#guard_msgs in
+#print smallFoldMap._spec
+/-- info: def LeanSASTests.genericFoldMap_sas_1 : Nat :=
+List.foldl (fun acc n => acc + n) 0 (List.map (fun a => 5 + smallCode a) univFast) -/
+#guard_msgs in
+#print genericFoldMap_sas_1
+/-- info: LeanSASTests.smallFoldMap._spec.eq_thm : smallFoldMap._spec = smallFoldMap -/
+#guard_msgs in
+#check smallFoldMap._spec.eq_thm
+
+example : smallFoldMap._spec = smallFoldMap :=
+  smallFoldMap._spec.eq_thm
+
+end LeanSASTests
+
+namespace LeanSASExternalTests
+
+def inc (x : Nat) := x + 1
+
+end LeanSASExternalTests
+
+namespace LeanSASTests
+
+def usesExternal (x : Nat) :=
+  LeanSASExternalTests.inc (0 + x)
+
+#sas usesExternal
+/-- info: def LeanSASTests.usesExternal._spec : Nat → Nat :=
+fun x => LeanSASExternalTests.inc x -/
+#guard_msgs in
+#print usesExternal._spec
+
+def recursiveCount : Nat → Nat
+  | 0 => 0
+  | n + 1 => recursiveCount n + 1
+
+/-- error: #sas does not specialize recursive definitions yet: LeanSASTests.recursiveCount -/
+#guard_msgs in
+#sas recursiveCount
+
+def usesRecursiveCallee (x : Nat) :=
+  recursiveCount (0 + x)
+
+#sas usesRecursiveCallee
+/-- info: def LeanSASTests.usesRecursiveCallee._spec : Nat → Nat :=
+fun x => recursiveCount x -/
+#guard_msgs in
+#print usesRecursiveCallee._spec
+/-- info: LeanSASTests.usesRecursiveCallee._spec.eq_thm (x : Nat) : usesRecursiveCallee._spec x = usesRecursiveCallee x -/
+#guard_msgs in
+#check usesRecursiveCallee._spec.eq_thm
+
+example (x : Nat) : usesRecursiveCallee._spec x = usesRecursiveCallee x :=
+  usesRecursiveCallee._spec.eq_thm x
+
+def matchCallee : Nat → Nat
+  | 0 => 10
+  | n + 1 => addWrap 0 n
+
+def usesMatchCallee (x : Nat) :=
+  matchCallee (0 + x)
+
+#sas usesMatchCallee
+/-- info: def LeanSASTests.usesMatchCallee._spec : Nat → Nat :=
+fun x => matchCallee._spec x -/
+#guard_msgs in
+#print usesMatchCallee._spec
+/--
+info: def LeanSASTests.matchCallee._spec : Nat → Nat :=
+fun x =>
+  match x with
+  | 0 => 10
+  | n.succ => addWrap_sas_1 n
+-/
+#guard_msgs in
+#print matchCallee._spec
+/--
+info: def LeanSASTests.addWrap_sas_1 : Nat → Nat :=
+fun x => x
+-/
+#guard_msgs in
+#print addWrap_sas_1
+/-- info: LeanSASTests.usesMatchCallee._spec.eq_thm (x : Nat) : usesMatchCallee._spec x = usesMatchCallee x -/
+#guard_msgs in
+#check usesMatchCallee._spec.eq_thm
+
+example (x : Nat) : usesMatchCallee._spec x = usesMatchCallee x :=
+  usesMatchCallee._spec.eq_thm x
+
 end LeanSASTests
 
 def main : IO Unit :=
